setting up the main lemma for finishing encrypt, for synch with aseem

examples/low-level/crypto/Crypto.AEAD.Encrypt.fst
@@ -52,24 +52,108 @@ val encrypt:
    plainlen: txtlen_32 {safelen i (v plainlen) (otp_offset i)} ->
       plain: plainBuffer i (v plainlen) ->
  cipher_tag: lbuffer (v plainlen + v MAC.taglen) ->
-        ST  unit
- (requires (fun h ->
-	enc_dec_separation st aad plain cipher_tag /\
-	enc_dec_liveness st aad plain cipher_tag h /\
-	fresh_nonce_st n st h /\
-	inv st h))
-  (ensures (fun h0 _ h1 ->
-	enc_dec_liveness st aad plain cipher_tag h1 /\
-	inv st h1 /\
-	encrypt_ensures st n aad plain cipher_tag h0 h1 /\
-	HS.modifies_transitively (Set.as_set [st.log_region; Buffer.frameOf cipher_tag]) h0 h1))
-	
+         ST  unit
+  (requires (fun h ->
+	     enc_dec_separation st aad plain cipher_tag /\
+	     enc_dec_liveness st aad plain cipher_tag h /\
+	     fresh_nonce_st n st h /\
+	     inv st h))
+   (ensures (fun h0 _ h1 ->
+	     enc_dec_liveness st aad plain cipher_tag h1 /\
+	     inv st h1 /\
+	     encrypt_ensures st n aad plain cipher_tag h0 h1 /\
+	     HS.modifies_transitively (Set.as_set [st.log_region; Buffer.frameOf cipher_tag]) h0 h1))
+
+
+assume //NS: boring, this should be in the buffer library
+val to_seq_temp: #a:Type -> b:Buffer.buffer a -> l:UInt32.t{v l <= Buffer.length b} -> ST (Seq.seq a)
+  (requires (fun h -> Buffer.live h b))
+  (ensures  (fun h0 r h1 -> h0 == h1 /\ Buffer.live h1 b /\ r == Buffer.as_seq h1 b))
+
+#reset-options "--z3rlimit 40 --initial_fuel 0 --max_fuel 0 --initial_ifuel 0 --max_ifuel 0"
+let ideal_ensures
+	 (#i: id)
+ 	 (st: aead_state i Writer)
+          (n: Cipher.iv (alg i))
+    (#aadlen: aadlen_32)
+        (aad: lbuffer (v aadlen))
+  (#plainlen: txtlen_32)
+      (plain: plainBuffer i (v plainlen))
+  (cipher_tag: lbuffer (v plainlen + v MAC.taglen){safeMac i})
+       (h0 h1: mem) = 
+    enc_dec_liveness st aad plain cipher_tag h0 /\
+    enc_dec_liveness st aad plain cipher_tag h1 /\
+    HS.modifies (Set.as_set [st.log_region]) h0 h1 /\
+    HS.modifies_ref st.log_region (TSet.singleton (HS.as_aref (st_ilog st))) h0 h1 /\ (
+    let entry = AEADEntry n (Buffer.as_seq h0 aad) 
+ 			    (v plainlen)
+			    (Plain.sel_plain h0 plainlen plain)
+			    (Buffer.as_seq h0 cipher_tag) in
+    let log = st_ilog st in 				      
+    HS.sel h1 log == SeqProperties.snoc (HS.sel h0 log) entry)
+
+assume val reestablish_inv:
+          i: id -> 
+         st: aead_state i Writer ->
+          n: Cipher.iv (alg i) ->
+    #aadlen: aadlen_32 ->
+        aad: lbuffer (v aadlen) ->
+  #plainlen: txtlen_32 {safelen i (v plainlen) (otp_offset i)} ->
+      plain: plainBuffer i (v plainlen) ->
+ cipher_tag: lbuffer (v plainlen + v MAC.taglen) ->
+         ak: CMA.state (i, n) -> 
+        acc: CMA.accBuffer (i, n) ->
+         h0: mem ->
+         h1: mem ->
+         h2: mem ->
+         h3: mem ->       
+         h4: mem ->               
+      Lemma 
+  (requires  (let cipher : lbuffer (v plainlen) = Buffer.sub cipher_tag 0ul plainlen in
+              let x_1 = {iv=n; ctr=otp_offset i} in
+              enc_dec_separation st aad plain cipher_tag  /\
+              enc_dec_liveness st aad plain cipher_tag h0 /\
+              enc_dec_liveness st aad plain cipher_tag h1 /\
+              enc_dec_liveness st aad plain cipher_tag h2 /\
+              enc_dec_liveness st aad plain cipher_tag h3 /\
+              inv st h0 /\
+              Enxor.enxor_invariant st.prf x_1 plainlen plainlen plain cipher h0 h1 /\
+              Enxor.modifies_table_above_x_and_buffer st.prf x_1 cipher h0 h1 /\
+              EncodingWrapper.accumulate_modifies_nothing h1 h2 /\
+              CMAWrapper.mac_ensures i n st aad plain cipher_tag ak acc h2 h3 /\ (
+              if safeMac i
+              then ideal_ensures st n aad plain cipher_tag h3 h4
+              else h3 == h4)))
+  (ensures    (inv st h4))
+
+val do_ideal:
+	 #i: id -> 
+ 	 st: aead_state i Writer ->
+          n: Cipher.iv (alg i) ->
+    #aadlen: aadlen_32 ->
+        aad: lbuffer (v aadlen) ->
+  #plainlen: txtlen_32 ->
+      plain: plainBuffer i (v plainlen) ->
+ cipher_tag: lbuffer (v plainlen + v MAC.taglen){safeMac i} ->
+         ST  unit
+ (requires (fun h -> 
+	    enc_dec_liveness st aad plain cipher_tag h))
+ (ensures  (fun h0 _ h1 ->
+	    ideal_ensures st n aad plain cipher_tag h0 h1))
+let do_ideal #i st n #aadlen aad #plainlen plain cipher_tag =
+    let ad = to_seq_temp aad aadlen in
+    let p = Plain.load plainlen plain in 
+    let c_tagged = to_seq_temp cipher_tag plainlen in
+    let entry = AEADEntry n ad (v plainlen) p c_tagged in
+    FStar.ST.recall (st_ilog st);
+    st_ilog st := SeqProperties.snoc !(st_ilog st) entry
+
 let encrypt i st n aadlen aad plainlen plain cipher_tagged =
   assume (plainlen <> 0ul); //TODO: remove this; currently cannot encrypt empty plain texts
   let h_init = get() in
   push_frame(); 
-  let h0 = get () in
-  frame_inv_push st h_init h0; //inv st h0
+  let h00 = get () in
+  frame_inv_push st h_init h00; //inv st h0
 
   let cipher : lbuffer (v plainlen) = Buffer.sub cipher_tagged 0ul plainlen in
   let tag = Buffer.sub cipher_tagged plainlen MAC.taglen in
@@ -77,30 +161,29 @@ let encrypt i st n aadlen aad plainlen plain cipher_tagged =
 
   //call prf_mac: get a mac key, ak
   let ak = PRF_MAC.prf_mac_enc st aad plain cipher_tagged st.ak x_0 in  // used for keying the one-time MAC
+  let h0 = get () in
+  let open CMA in 
+  
+  //call enxor: fragment the plaintext, call the prf, and fill in the cipher text
+  Enxor.enxor n st aad plain cipher_tagged ak;
   let h1 = get () in
 
-  //call enxor: fragment the plaintext, call the prf, and fill in the cipher text
-  Enxor.enxor n st aad plain cipher_tagged;
-  let h2 = get () in
+  (* assume (EncodingWrapper.ak_aad_cipher_separate ak aad cipher_tagged); //slow *)
 
-  assume (PRF_MAC.ak_live st.prf.mac_rgn ak h2); //provable, but slow
-
-  //call accumulate: encode the ciphertext and additional data for mac'ing 
+  //call accumulate: encode the ciphertext and additional data for mac'ing
   let acc = EncodingWrapper.accumulate_enc #(i, n) st ak aad plain cipher_tagged in
   
-  let h3 = get () in
-  admit()
-  
-  Buffer.lemma_reveal_modifies_0 h2 h3;
+  let h2 = get () in
+
+  (* assume(verify_liveness ak tag h2); //slow *)
+
   //call mac: filling in the tag component of the out buffer
-  mac_wrapper #(i,n) ak acc tag;
+  CMAWrapper.mac #(i,n) st aad plain cipher_tagged ak acc h1;
+  let h3 = get () in 
+  
+  if safeMac i 
+  then do_ideal st n aad plain cipher_tagged;
+  let h4 = get () in
+  let x_1 = PRF.incr i x_0 in
+  reestablish_inv i st n aad plain cipher_tagged ak acc h0 h1 h2 h3 h4;
   admit()
-
-(* (\* start: ideal and proof steps, to finish up, notably writing to the AEAD table  *\) *)
-(*   finish_after_mac h0 h3 i st n aadlen aad plainlen plain cipher_tagged ak acc tag; *)
-(* (\* end *\) *)
-
-(*   let h5 = get () in   *)
-(*   pop_frame(); //clean up any local allocation on our stack *)
-(*   encrypt_ensures_push_pop i st n aadlen aad plainlen plain cipher_tagged h_init h0 h5 *)
-
